\documentclass[12pt]{article}
\usepackage[a4paper, total={7in, 10in}]{geometry}
\usepackage{amsmath}
\usepackage{graphicx}

\title{AM-GM Inequality Lesson\vspace{-3mm}}
\author{2018-2019 SLSS Math Club\vspace{-5mm}}
\date{February 6, 2019\vspace{-5mm}}

\begin{document}
\maketitle

\section{Definitions}
\subsection{Arithmetic Mean}
A type of mean, calculated as the sum of $n$ numbers divided by $n$.
$$\text{AM} = \frac{a_{1} + a_{2} + \dots + a_{n - 1} + a_{n}}{n}$$

\subsection{Geometric Mean}
A type of mean, calculated as the $n$-th root of the product of $n$ numbers. $$\text{GM} = \sqrt[n]{a_{1} a_{2} \dots a_{n - 1} a_{n}}$$

\subsection{Arithmetic Mean - Geometric Mean Inequality}
States that the arithmetic mean of a given set is equal to or greater than the geometric mean of the same set if all elements are non-negative ($a_i \geq 0$)

\begin{align*}
    \text{AM} & \geq \text{GM} \\
     \frac{a_{1} + a_{2} + \dots + a_{n - 1} + a_{n}}{n} & \geq \sqrt[n]{a_{1} a_{2} \dots a_{n - 1} a_{n}}
\end{align*}

\subsubsection*{Equality Case}
Arithmetic and geometric means are equal if and only if all elements are identical. $$a_{1} = a_{2} = \dots = a_{n - 1} = a_{n}$$

\newpage

\section{Applications}
\subsection{Proving Inequalities}
\subsubsection*{Example}
Prove the following inequality: $$2a^3 + b^3 \geq 3a^2b$$ $\forall x, y > 0$.

\subsubsection*{Solution}
We can rewrite the $\text{LHS}$ of the equation as follows: $$2a^3 + b^3 = a^3 + a^3 + b^3$$
Applying AM-GM Inequality:
\begin{align*}
    \text{AM} &= \frac{a^3 + a^3 + b^3}{3} \\
    \text{GM} &= \sqrt[3]{a^3 a^3 b^3} \\
              &= a^2 b \\
  \frac{a^3 + a^3 + b^3}{3} &\geq a^2 b \\
  2a^3 + b^3 &\geq 3a^2 b
\end{align*} 
Therefore, via AM-GM Inequality, $2a^3 + b^3 \geq 3a^2 b$, as desired.

\subsection{Simplifying Equations}
\subsubsection*{Example}
Let $a = 10$, solve for $b$ and $c$ if $$(a + b + c)^3 = 27abc$$

\subsubsection*{Solution}
Rearranging the equation, we achieve the following:
\begin{align*}
    (a + b + c)^3 = 27abc \\
    a + b + c = 3 \sqrt[3]{abc} \\
    \frac{a + b + c}{3} = \sqrt[3]{abc}
\end{align*}
Knowing that the equality case of AM-GM Inequality occurs if and only if $$a = b = c$$, our equality can be simplified to $a = b = c$ or $b = c = 10$

\subsection{Determining Minimum Value}
\subsubsection*{Example}
Determine the minimum value of $$x^2 + 4xy + 4y^2 + 2z^3$$ if $x, y, z \geq 0$ and $xyz = 32$.

\subsubsection*{Solution}
Applying AM-GM Inequality, we achieve the following:
\begin{align*}
    \frac{x^2 + 4xy + 4y^2 + 2z^3}{4} &\geq \sqrt[4]{(x^2)(4xy)(4y^2)(2z^3)} \\
    x^2 + 4xy + 4y^2 + 2z^3 &\geq 4 \sqrt[4]{(x^2)(4xy)(4y^2)(2z^3)} \\
    x^2 + 4xy + 4y^2 + 2z^3 &\geq \sqrt[4]{32x^3y^3z^3} \\
    x^2 + 4xy + 4y^2 + 2z^3 &\geq \sqrt[4]{32(32)^3} \\
    x^2 + 4xy + 4y^2 + 2z^3 &\geq 32
\end{align*}
Therefore, the minimum value of $x^2 + 4xy + 4y^2 + 2z^3$ is $32$.

\subsection{Determining Maximum Value}
\subsubsection*{Example}
Determine the maximum value of $$4xy - x^2y - xy^2$$

\subsubsection*{Solution}
Factoring our equation and applying AM-GM Inequality, we achieve the following:
\begin{align*}
    &= 4xy - x^2y - xy^2 \\
    &= xy(4 - x - y) \\
    \frac{x + y + (4 - x - y)}{3} \geq \sqrt[3]{xy(4 - x - y)} \\
    \frac{4}{3} \geq \sqrt[3]{xy(4 - x - y)} \\
    \frac{64}{9} \geq xy(4 - x - y)
\end{align*}
Therefore, the maximum value of $xy(4 - x - y)$ is $\frac{64}{9}$

\end{document}